kuiops/common/supergemm/mm_splitk/Kuiops.SuperGEMM.Mm.SplitK.Output.fst
@@ -6,7 +6,9 @@ open Kuiper
 open Kuiper.Tensor
 open Kuiper.Tensor.Tiling
 open Kuiper.Kernel.GEMM.Tiled.Common.Vec { block_tile, warp_tile }
-open Kuiper.Kernel.GEMM.TensorCore2D.KernelDesc { warp_tile_pts_to }
+open Kuiper.Kernel.GEMM.TensorCore2D.KernelDesc { warp_tile_pts_to, warp_tile_approximates }
+open Kuiper.Kernel.GEMM.TensorCore2D.To.EpilogueState { epilogue_warp_input }
+open Kuiops.SuperGEMM.Mm.SplitK.Gather
 open Kuiper.EMatrix.Tiling { ematrix_subtile }
 
 module SZ = Kuiper.SizeT
@@ -209,5 +211,132 @@ fn gather_ws_warps
       exists* (em : chest2 et (SZ.v bm) (SZ.v bn)).
         array2_subtile gW (SZ.v bm) (SZ.v bn) br bc |-> em);
   array2_untile_underspec gW (SZ.v bm) (SZ.v bn) #1.0R;
+}
+#pop-options
+
+#push-options "--z3rlimit 15 --fuel 1 --ifuel 1 --split_queries always"
+ghost
+fn gather_ws_approximates
+  (#et : Type0) {| scalar et |} {| real_like et |}
+  (#mm #nn : szp)
+  (#lW : layout2 (SZ.v mm) (SZ.v nn)) {| T.ctlayout lW |}
+  (gW : array2 et lW)
+  (bm bn tm tn wm wn : szp)
+  (#_ : squash (bm /?+ mm /\ bn /?+ nn /\
+                wm * tm /?+ bm /\ wn * tn /?+ bn /\
+                tm /?+ bm /\ tn /?+ bn))
+  (#_ : squash (SZ.fits lW.ulen))
+  (nblk : szp{SZ.v nblk == SZ.v mm / SZ.v bm * (SZ.v nn / SZ.v bn)})
+  (nthr : szp{SZ.v nthr == SZ.v bm / (SZ.v wm * SZ.v tm) * (SZ.v bn / (SZ.v wn * SZ.v tn)) * warp_size})
+  (rW : chest2 real (SZ.v mm) (SZ.v nn))
+  ()
+  requires
+    forall+ (bid : natlt nblk) (tid : natlt nthr).
+      ws_warp_approximates gW bm bn tm tn wm wn bid tid rW
+  ensures
+    exists* (eW : chest2 et (SZ.v mm) (SZ.v nn)).
+      gW |-> eW ** pure (eW %~ rW)
+{
+  forevery_map
+    (fun (bid : natlt nblk) ->
+      forall+ (tid : natlt nthr).
+        ws_warp_approximates gW bm bn tm tn wm wn bid tid rW)
+    (fun (bid : natlt nblk) ->
+      exists* (em : chest2 et (SZ.v bm) (SZ.v bn)).
+        block_tile gW (SZ.v bm) (SZ.v bn) bid |-> em **
+        pure (em %~ ematrix_subtile rW (SZ.v bm) (SZ.v bn)
+                      (bid / (nn / bn)) (bid % (nn / bn))))
+    fn bid {
+      let wBlock = block_tile gW (SZ.v bm) (SZ.v bn) bid;
+      forevery_map
+        (fun (tid : natlt nthr) ->
+          ws_warp_approximates gW bm bn tm tn wm wn bid tid rW)
+        (fun (tid : natlt nthr) ->
+          exists* (em : chest2 et (wm * tm) (wn * tn)).
+            warp_tile wBlock (wm * tm) (wn * tn) (tid / warp_size)
+              |-> Frac (1.0R /. warp_size) em **
+            pure (em %~ ematrix_subtile
+                          (ematrix_subtile rW (SZ.v bm) (SZ.v bn)
+                            (bid / (nn / bn)) (bid % (nn / bn)))
+                          (wm * tm) (wn * tn)
+                          ((tid / warp_size) / (bn / (wn * tn)))
+                          ((tid / warp_size) % (bn / (wn * tn)))))
+        fn tid {
+          unfold (ws_warp_approximates gW bm bn tm tn wm wn bid tid rW);
+          unfold (warp_tile_approximates gW bm bn tm tn wm wn bid (tid / warp_size)
+                   (epilogue_warp_input rW bm bn tm tn wm wn bid tid));
+          with em. assert (warp_tile_pts_to gW bm bn tm tn wm wn bid (tid / warp_size) em);
+          unfold (warp_tile_pts_to gW bm bn tm tn wm wn bid (tid / warp_size) em);
+          rewrite each
+            warp_tile (block_tile gW (SZ.v bm) (SZ.v bn) bid) (wm * tm) (wn * tn) (tid / warp_size)
+          as warp_tile wBlock (wm * tm) (wn * tn) (tid / warp_size);
+        };
+      forevery_factor' nthr
+        (bm / (wm * tm) * (bn / (wn * tn))) warp_size
+        (fun (wid : natlt (bm / (wm * tm) * (bn / (wn * tn)))) (lane : natlt warp_size) ->
+          exists* (em : chest2 et (wm * tm) (wn * tn)).
+            warp_tile wBlock (wm * tm) (wn * tn) wid
+              |-> Frac (1.0R /. warp_size) em **
+            pure (em %~ ematrix_subtile
+                          (ematrix_subtile rW (SZ.v bm) (SZ.v bn)
+                            (bid / (nn / bn)) (bid % (nn / bn)))
+                          (wm * tm) (wn * tn)
+                          (wid / (bn / (wn * tn))) (wid % (bn / (wn * tn)))));
+      forevery_map
+        (fun (wid : natlt (bm / (wm * tm) * (bn / (wn * tn)))) ->
+          forall+ (lane : natlt warp_size).
+            exists* (em : chest2 et (wm * tm) (wn * tn)).
+              warp_tile wBlock (wm * tm) (wn * tn) wid
+                |-> Frac (1.0R /. warp_size) em **
+              pure (em %~ ematrix_subtile
+                            (ematrix_subtile rW (SZ.v bm) (SZ.v bn)
+                              (bid / (nn / bn)) (bid % (nn / bn)))
+                            (wm * tm) (wn * tn)
+                            (wid / (bn / (wn * tn))) (wid % (bn / (wn * tn)))))
+        (fun (wid : natlt (bm / (wm * tm) * (bn / (wn * tn)))) ->
+          exists* (em : chest2 et (wm * tm) (wn * tn)).
+            array2_subtile wBlock (wm * tm) (wn * tn)
+              (wid / (bn / (wn * tn))) (wid % (bn / (wn * tn)))
+              |-> em **
+            pure (em %~ ematrix_subtile
+                          (ematrix_subtile rW (SZ.v bm) (SZ.v bn)
+                            (bid / (nn / bn)) (bid % (nn / bn)))
+                          (wm * tm) (wn * tn)
+                          (wid / (bn / (wn * tn))) (wid % (bn / (wn * tn)))))
+        fn wid {
+          array2_gather_n_approximates (warp_tile wBlock (wm * tm) (wn * tn) wid)
+            warp_size #1.0R
+            (ematrix_subtile
+              (ematrix_subtile rW (SZ.v bm) (SZ.v bn)
+                (bid / (nn / bn)) (bid % (nn / bn)))
+              (wm * tm) (wn * tn)
+              (wid / (bn / (wn * tn))) (wid % (bn / (wn * tn))));
+          rewrite each warp_tile wBlock (wm * tm) (wn * tn) wid
+          as array2_subtile wBlock (wm * tm) (wn * tn)
+               (wid / (bn / (wn * tn))) (wid % (bn / (wn * tn)));
+        };
+      forevery_factor'
+        (bm / (wm * tm) * (bn / (wn * tn)))
+        (bm / (wm * tm))
+        (bn / (wn * tn))
+        (fun (wr : natlt (bm / (wm * tm))) (wc : natlt (bn / (wn * tn))) ->
+          exists* (em : chest2 et (wm * tm) (wn * tn)).
+            array2_subtile wBlock (wm * tm) (wn * tn) wr wc |-> em **
+            pure (em %~ ematrix_subtile
+                          (ematrix_subtile rW (SZ.v bm) (SZ.v bn)
+                            (bid / (nn / bn)) (bid % (nn / bn)))
+                          (wm * tm) (wn * tn) wr wc));
+      array2_untile_approximates wBlock (wm * tm) (wn * tn)
+        (ematrix_subtile rW (SZ.v bm) (SZ.v bn)
+          (bid / (nn / bn)) (bid % (nn / bn)));
+      rewrite each wBlock as
+        array2_subtile gW (SZ.v bm) (SZ.v bn) (bid / (nn / bn)) (bid % (nn / bn));
+    };
+  forevery_factor' nblk (mm / bm) (nn / bn)
+    (fun (br : natlt (mm / bm)) (bc : natlt (nn / bn)) ->
+      exists* (em : chest2 et (SZ.v bm) (SZ.v bn)).
+        array2_subtile gW (SZ.v bm) (SZ.v bn) br bc |-> em **
+        pure (em %~ ematrix_subtile rW (SZ.v bm) (SZ.v bn) br bc));
+  array2_untile_approximates gW (SZ.v bm) (SZ.v bn) rW;
 }
 #pop-options
